share/steel/examples/steel/dplex/Domain.Steel.fst
@@ -1,0 +1,26 @@
+module Domain.Steel
+
+module M  = Model
+module TC = Selectors.Tree.Core
+module T  = Trees
+
+open Steel.Memory
+open Steel.Effect.Atomic
+open Steel.Effect
+
+// A Steel reference to a model
+let model_ref = TC.t (T.node_data M.field_key M.field_value)
+
+// Pure equality lifted to Steel via selector
+val model_eqb
+  (ptr1 ptr2: model_ref)
+  : Steel bool
+    (TC.linked_tree ptr1 `star` TC.linked_tree ptr2)
+    (fun _ -> TC.linked_tree ptr1 `star` TC.linked_tree ptr2)
+    (requires fun _ -> True)
+    (ensures fun h0 b h1 ->
+      TC.v_linked_tree ptr1 h0 == TC.v_linked_tree ptr1 h1 /\
+      TC.v_linked_tree ptr2 h0 == TC.v_linked_tree ptr2 h1 /\
+      b == M.model_eqb
+             (TC.v_linked_tree ptr1 h0)
+             (TC.v_linked_tree ptr2 h0))
